\documentclass[11pt]{article}
\usepackage{amsmath}
\usepackage[width=7.5in,height=9.5in]{geometry}

\newcommand{\ds}{\displaystyle}
\newcommand{\tr}{\operatorname{tr}}

\begin{document}
\pagestyle{empty}
\section*{Formula Sheet} %%% FORMULA SHEET FOR MIDTERM 3 
\hrule

~
\subsection*{Quadratic Formula}
$$x = \frac{-b \pm \sqrt{ b^2 - 4 ac }}{2a}$$


\subsection*{Integrating Factors}

A first order linear differential equation $\dfrac{dy}{dt} + f(t) y = g(t)$ has general solution 
$$y(t) = \frac{\int e^{F(t)} g(t) \, dt}{e^{F(t)}}$$
where $F(t)$ is any antiderivative of $f(t)$.

%\subsection*{Characteristic Polynomial for 2-by-2 Matrices}
%$$\det(A - \lambda I) = \lambda^2 - (\tr A) \lambda + \det A.$$

\subsection*{Trace-Determinant Formula for the Characteristic Polynomial}
For a 2-by-2 matrix $A$, the characteristic polynomial is
$$\lambda^2 - \lambda \tr A  + \det A.$$

\subsection*{Linear Systems} 

For a linear system $\dfrac{d\mathbf{x}}{dt} = A \mathbf{x}$:

\begin{center}
\begin{tabular}{|c|c|}
\hline

\begin{minipage}{0.4\textwidth}
\bigskip
\textbf{Straight-line solutions} 
$$\mathbf{x}(t) = C e^{\lambda t} \mathbf{v}.$$
\bigskip
\end{minipage}

& 

\begin{minipage}{0.4\textwidth}
\bigskip
\textbf{Matrix exponential solution}
$$\mathbf{x}(t) = e^{At} \mathbf{x}(0).$$
\bigskip
\end{minipage}

\\ \hline

\begin{minipage}{0.4\textwidth}
\bigskip
\item \textbf{Complex eigenvalues} \\

If $\lambda = \alpha \pm i \beta$ is a complex eigenvalue with eigenvector $\mathbf{v}$, then the real and imaginary parts of 
$$e^{\alpha t} (\cos (\beta t) \pm i \sin (\beta t)) \mathbf{v}$$
are both real-valued solutions.
\bigskip
\end{minipage}

& 


\begin{minipage}{0.4\textwidth}
\bigskip
\item \textbf{Repeated eigenvalues} \\

If $A$ is a 2-by-2 matrix with a repeated eigenvalue $\lambda$, then the solution is

$$\mathbf{x}(t) = e^{\lambda t} (I + t(A-\lambda I)) \mathbf{x}(0).$$


\bigskip
\end{minipage}


\\ \hline
\end{tabular}

\end{center}

\subsection*{Hamiltonian Systems}
\begin{align*}
\dfrac{dx}{dt} &= \dfrac{\partial H}{\partial y} \\
\dfrac{dy}{dt} &= -\dfrac{\partial H}{\partial x}
\end{align*}

\end{document}
